Finish RCC implementation using linear env

RCC.v
@@ -20,20 +20,26 @@ Module Type RCC.
   Parameter locked : forall {l:lock}, hpred (lockwitness l).
   Parameter unlocked : forall {l:lock}, hpred (lockwitness l).
 
-  (** Note that the witness arguments should really be monadic in the implementation; I'm prototyping
-      actual source code. I'm also making them explicit, because they aren't inferred normally, but
-      are inferred when using Program. *)
-  Parameter rcc_read : forall {A B P R G}`{rel_fold A}{l:lock}(w:ref{lockwitness l | locked}[empty,locked-->unlocked])(r:rccref A P R G l),
-                              hreflexive G -> rgfold R G = B -> B.
+  (** Because the witness will always be in the linear context, we can't just re-export a pure
+      read.  Unfortunately this pushes all RCC reads into imperative land, where proofs are less
+      pleasant / direct. *)
+  Parameter rcc_read : forall {Γ A B P R G}`{rel_fold A}{l:lock}{w:var}{pf:tymember w (ref{lockwitness l | locked}[empty,locked-->unlocked]) Γ}(r:rccref A P R G l),
+                              hreflexive G -> rgfold R G = B -> rgref Γ B Γ.
   (** We expose hwrite, because we need a way for clients to prove obligations that this module
       must translate down to the real RGref primitives, but without exposing the fact that
       rccrefs are just rgrefs.  This means re-exporting some axioms needed to state client obligations. *)
   Parameter hwrite : forall {l A P R G} (p:rccref A P R G l) (v:A) (h:heap), heap.
-  Parameter rcc_write : forall {Γ A}`{rel_fold A}{P R G}`{hreflexive G}{l:lock}(w:ref{lockwitness l | locked}[empty,locked-->unlocked])(x:rccref A P R G l)(e:A)
+(*  Parameter rcc_write : forall {Γ A}`{rel_fold A}{P R G}`{hreflexive G}{l:lock}{w:var}{pf:tymember w (ref{lockwitness l | locked}[empty,locked-->unlocked]) Γ}(x:rccref A P R G l)(e:A)
                                (meta_x:A)(meta_e:A) (* meta args *)
                                {guar:forall h, (forall A (fa:rel_fold A), fa = meta_fold) -> G (meta_x) e h (hwrite x e h)}
                                {pres:(forall h, P meta_x h -> P meta_e (hwrite x meta_e h))}
                                , rgref Γ unit Γ.
+*)
+  Parameter rcc_write : forall {Γ Γ'}{A:Set}`{rel_fold A}{P R G}`{hreflexive G}{l:lock}{w:var}{pf:tymember w (ref{lockwitness l | locked}[empty,locked-->unlocked]) Γ}(x:rccref A P R G l)(e:rgref Γ A Γ')
+                               (meta_x_deref:rgref Γ A Γ') (meta_e_fold:rgref Γ A Γ')
+                               {guar:forall h env, G (valueOf _ _ _ env h meta_x_deref) (valueOf _ _ _ env h e) h (hwrite x (valueOf _ _ _ env h e) h)}
+                               {pres:(forall h env, P (valueOf _ _ _ env h meta_x_deref) h -> P (valueOf _ _ _ env h meta_e_fold) (hwrite x (valueOf _ _ _ env h meta_e_fold) h))}
+                               , rgref Γ unit Γ'.
 
   Parameter rcc_alloc : forall {Γ}{T:Set}{RT:ImmediateReachability T}{CT:Containment T}{FT:rel_fold T} P R G (l:lock) (e:T), 
                 stable P R ->        (* predicate is stable *)
@@ -44,8 +50,8 @@ Module Type RCC.
                 rgref Γ (rccref T P R G l) Γ.
   (** Both of these should be introducing and removing witnesses in the linear context.  Since that's
       currently not implemented, for this sketch we're going closer to the desired source language. *)
-  Parameter acquire : forall {Γ}(l:lock), rgref Γ (ref{lockwitness l | locked}[empty,locked-->unlocked]) Γ.
-  Parameter release : forall {Γ}{l:lock}, ref{lockwitness l | locked}[empty,locked-->unlocked] -> rgref Γ unit Γ.
+  Parameter acquire : forall {Γ}(w:var)(l:lock), rgref Γ unit (w:ref{lockwitness l | locked}[empty,locked-->unlocked],Γ).
+  Parameter release : forall {Γ}{l:lock}(w:var){pf:(tymember w (ref{lockwitness l | locked}[empty,locked-->unlocked]) Γ)}, rgref Γ unit (tyrem pf).
 End RCC.
 (** TODO: define folding over rcc refs *)
 (** * A Partial RCC Implementation *)
@@ -59,16 +65,23 @@ Module RCCImpl : RCC.
 
   (** Note that the witness arguments should really be monadic in the implementation; I'm prototyping
       actual source code.  Sort of... still using the monadic return type... *)
-  Program Definition rcc_read {A B P R G}`{rel_fold A}{l:lock}(w:ref{lockwitness l | locked}[empty,locked-->unlocked])(r:rccref A P R G l)
-                      (hrefl:hreflexive G)(fold:rgfold R G = B) := deref hrefl fold r.
+  Program Definition rcc_read {Γ A B P R G}`{rel_fold A}{l:lock}{w:var}{pf:tymember w (ref{lockwitness l | locked}[empty,locked-->unlocked]) Γ}(r:rccref A P R G l)
+                      (hrefl:hreflexive G)(fold:rgfold R G = B) : rgref Γ B Γ := read_imp Γ A B _ _ _ _ _ _ r.
+
   Definition hwrite := fun l:lock => @heap_write.
   (** Clients prove goals over the abstracted rcc reads; the module internally converts those for write's use *)
-  Program Definition rcc_write {Γ A}`{rel_fold A}{P R G}`{hreflexive G}{l:lock}(w:ref{lockwitness l | locked}[empty,locked-->unlocked])(x:rccref A P R G l)(e:A)
+(*  Program Definition rcc_write {Γ A}`{rel_fold A}{P R G}`{hreflexive G}{l:lock}(w:var){pf:tymember w (ref{lockwitness l | locked}[empty,locked-->unlocked]) Γ}(x:rccref A P R G l)(e:A)
                                (meta_x:A)(meta_e:A) (* meta args *)
                                {guar:forall h, (forall A (fa:rel_fold A), fa = meta_fold) -> G (meta_x) e h (heap_write x e h)}
                                {pres:(forall h, P meta_x h -> P meta_e (heap_write x meta_e h))}
                                : rgref Γ unit Γ :=
-      @write' Γ A _ P R G _ x e meta_x meta_e _ _.
+      @write' Γ A _ P R G _ x e meta_x meta_e _ _.*)
+  Program Definition rcc_write {Γ Γ'}{A:Set}`{rel_fold A}{P R G}`{hreflexive G}{l:lock}{w:var}{pf:tymember w (ref{lockwitness l | locked}[empty,locked-->unlocked]) Γ}(x:rccref A P R G l)(e:rgref Γ A Γ')
+                               (meta_x_deref:rgref Γ A Γ') (meta_e_fold:rgref Γ A Γ')
+                               {guar:forall h env, G (valueOf _ _ _ env h meta_x_deref) (valueOf _ _ _ env h e) h (hwrite l _ _ _ _ x (valueOf _ _ _ env h e) h)}
+                               {pres:(forall h env, P (valueOf _ _ _ env h meta_x_deref) h -> P (valueOf _ _ _ env h meta_e_fold) (hwrite _ _ _ _ _ x (valueOf _ _ _ env h meta_e_fold) h))}
+                               : rgref Γ unit Γ' :=
+                               @write_imp_exp Γ Γ' A _ P R G _ x e meta_x_deref meta_e_fold guar pres.
 
   Program Definition rcc_alloc {Γ}{T:Set}{RT:ImmediateReachability T}{CT:Containment T}{FT:rel_fold T} P R G (l:lock) (e:T) 
                 `(stable P R)        (* predicate is stable *)
@@ -78,9 +91,8 @@ Module RCCImpl : RCC.
                 `(precise_rel G)     (* G precise *)
                 : rgref Γ (rccref T P R G l) Γ :=
       alloc _ _ _ e _ _ _ _ _.
-
-  Parameter acquire : forall {Γ}(l:lock), rgref Γ (ref{lockwitness l | locked}[empty,locked-->unlocked]) Γ.
-  Parameter release : forall {Γ}{l:lock}, ref{lockwitness l | locked}[empty,locked-->unlocked] -> rgref Γ unit Γ.
+  Parameter acquire : forall {Γ}(w:var)(l:lock), rgref Γ unit (w:ref{lockwitness l | locked}[empty,locked-->unlocked],Γ).
+  Parameter release : forall {Γ}{l:lock}(w:var){pf:(tymember w (ref{lockwitness l | locked}[empty,locked-->unlocked]) Γ)}, rgref Γ unit (tyrem pf).
 End RCCImpl.
 
 (** * Using the RCC Module : A race-free counter *)
@@ -95,23 +107,43 @@ Section RaceFreeMonotonicCounter.
     fun n n' _ _ => n <= n'.
 
   Hint Unfold increasing.
-  Local Obligation Tactic := intros; eauto with arith; compute; auto with arith.
+  Local Obligation Tactic := intros; eauto with arith; compute; auto with arith; repeat constructor.
 
   Program Definition rf_monotonic_counter (l:lock) := rccref nat any increasing increasing l.
-  Program Definition read_counter {l:lock}{w:ref{lockwitness l | locked}[empty,locked-->unlocked]}(c:rf_monotonic_counter l) : nat :=
-    @rcc_read _ _ _ _ _ _ l w c _ _.
+  Program Definition read_counter {Γ}{l:lock}{w:var}{pf:tymember w (ref{lockwitness l | locked}[empty,locked-->unlocked]) Γ}
+    (c:rf_monotonic_counter l) : rgref Γ nat Γ :=
+    @rcc_read _ _ _ _ _ _ _ l w _ c _ _.
   Check @rcc_write.
-  Program Definition inc_monotonic {Γ l}(w:ref{lockwitness l|locked}[empty,locked-->unlocked]) (p:rf_monotonic_counter l) : rgref Γ unit Γ :=
+  Local Obligation Tactic := intros; compute [increasing hreflexive]; eauto; try apply natsp.
+  Program Definition inc_monotonic {Γ l}{w:var}{pf:tymember w (ref{lockwitness l|locked}[empty,locked-->unlocked]) Γ} (p:rf_monotonic_counter l) : rgref Γ unit Γ :=
     (*rccwrite p <:= ((rcc_read p _ _) + 1).*)
-    @rcc_write Γ nat _ any increasing increasing _ l _ p (rcc_read _ p _ _ + 1) ({{{rcc_read _ p _ _}}}) ({{{rcc_read _ p _ _ + 1}}}) _ _.
+    (* We can't directly add to the read result because that result is monadic.  Instead we have to use pureApp. *)
+    @rcc_write Γ Γ nat _ any increasing increasing _ l _ _ p
+        (@pureApp _ _ _ _ _ (plus 1) (@rcc_read Γ _ _ _ _ _ _ l w pf p _ _))
+        ({{{@rcc_read Γ _ _ _ _ _ _ l w pf p _ _}}})
+        ({{{pureApp _ _ _ _ _ (plus 1) (@rcc_read Γ _ _ _ _ _ _ l w pf p _ _)}}}) _ _.
+  Next Obligation.
+    (* And again, tripped up by opacity of Program's obligation solutions... *)
+    unfold inc_monotonic_obligation_8. unfold inc_monotonic_obligation_6.
+    unfold inc_monotonic_obligation_5. unfold inc_monotonic_obligation_7.
+    unfold inc_monotonic_obligation_4.
+    (* Can't just do eauto with arith anymore, because we need to apply some axioms about the behavior of imperative code. *)
+    (* TODO: Double-check: we're using the same env for write checks that correspond to both before and after executing e,
+             which is only okay when Γ = Γ'... *)
+    apply weak_pureApp_morphism; eauto with arith.
+  Qed.
+
+  Local Obligation Tactic := intros; eauto with arith; compute; auto with arith; repeat constructor.
   Program Definition mkRFCounter {Γ} (l:lock) : rgref Γ (rf_monotonic_counter l) Γ :=
     (*RCCAlloc l 0.*)
     rcc_alloc _ _ _ l 0 _ _ _ _ _.
   (** Again, remember that the lock witness should really be in a monadic context *)
+  Parameter w : var.
   Program Example test_counter {Γ} (l:lock) : rgref Γ unit Γ :=
     x <- mkRFCounter l;
-    w <- acquire l;
-    _ <- inc_monotonic _ x;
-    release w.
+    _ <- acquire w l;
+    _ <- @inc_monotonic _ _ w _ x;
+    @release _ _ w _.
+
   
 End RaceFreeMonotonicCounter.
